---
uid: S000132
slug: duncan's-space
name: Duncan's space
counterexamples_id: 136
refs:
  - doi: 10.1007/978-1-4612-6290-9
    name: Counterexamples in Topology
---
Let $A$ be the set of all strictly increasing, infinite sequences of positive integers. For any $x\in A$, define $N(n,x)$ as the number of elements of $x$ less than $n$. Let $\delta (x) =\lim_{n\to\infty} \frac{N(n,x)}{n}$. Let $X$ be the subset of $A$ containing precisely the sequences, $x$, for which $\delta(x)$ exists. Now for any $x,y\in X$ define $k(x,y)$ to be the smallest index $i$ such that $x_i\neq y_i$. We define a metric $d(x,y)$ on $X$ as $$d(x,y)=\frac{1}{k(x,y)}+|\delta (x) - \delta (y)| \text{ with } d(x,x)=0.$$ Duncan's Space is the topology on $X$ induced by this metric.

Defined as counterexample #136 ("Duncan's Space")
in {{doi:10.1007/978-1-4612-6290-9}}.

<!-- [[Proof of Topology]]
To prove $d(x,y)$ is a metric on $X$, we must prove for every $x,y \in X$:
$d(x,x)=0$,
$d(x,y)>0$,
$d(x,y)=d(y,x)$, and
$d(x,y)+d(y,z)\geq d(x,z)$
By definition, $d(x,x)=0$.
Note that for all $x,y\in X$, $k(x,y)>0$, and clearly, $|\delta (x) - \delta (y)|>0$. It follows that $d(x,y)>0$.
Note, $k(x,y)=k(y,x)$ and $|\delta (x) - \delta (y)| = |\delta (y)-\delta (x)|$. So, $$d(x,y)=\frac{1}{k(x,y)}+|\delta (x) - \delta (y)|=\frac{1}{k(y,x)}+|\delta (y)-\delta (x)|=d(y,x).$$
For the final condition, we begin with the definition of our distance function. We must show $$\frac{1}{k(x,y)}+|\delta(x)-\delta(y)|+\frac{1}{k(y,z)}+|\delta(y)-\delta(z)|\geq \frac{1}{k(x,z)} +|\delta(x)-\delta(z)|.$$ It is sufficient to prove:
$$|\delta(x)-\delta(y)|+|\delta(y)-\delta(z)|\geq | \delta(x)-\delta(z)|$$
$$\frac{1}{k(x,y)}+\frac{1}{k(y,z)}\geq \frac{1}{k(x,z)}$$
To prove the first, we utilize the triangle inequality $|a|+|b|\geq |a+b|$ with $a=\delta(x)-\delta(y)$ and $b=\delta(y)-\delta(z)$. So, $$|\delta(x)-\delta(y)|+|\delta(y)-\delta(z)|\geq |\delta(x)-\delta(y)+\delta(y)-\delta(z)| = |\delta(x)-\delta(z)|.$$
Note that to prove the second, we will instead show that either $k(x,y) \text { or } k(y,z)$ is less than or equal to $k(x,z)$. It then will follow that the second holds. There are two cases:
$$\text{ Case 1: } k(x,y)\leq k(x,z)$$
This directly implies $$\frac{1}{k(x,y)}\geq\frac{1}{k(x,z)}.$$
$$\text{Case 2:} k(x,y)>k(x,z)$$
By definition, $x_n=y_n$ for $n<k(x,y)$, and $x_n=z_n$ for $n<k(x,z)$. Because $k(x,y)>k(x,z)$, it follows $x_n=y_n=z_n$ for $n<k(x,z)$. Furthermore, $x_{k(x,z)}\neq z_{k(x,z)}$, so $y_{k(x,z)}\neq z_{k(x,z)}$. Thus, $k(y,z)=k(x,z)$. -->
